Add evaln_substPartrec

Project/Substitute.lean
@@ -1,6 +1,7 @@
 module
 
 public import Project.Queries
+public import Project.PartrecCode
 public import Mathlib.Computability.Halting
 
 /-!
@@ -38,9 +39,9 @@ def subst (c : Code) (c' : Code) : Code := match c with
 | rfind' cf => rfind' (cf.subst c')
 
 /--
-Substitute the oracle in a code `c` for a `Nat.Partrec.Code` `c'`.
+Substitute the oracle in a code `c` for a `Partrec.Code` `c'`.
 -/
-def substPartrec (c : Code) (c' : Nat.Partrec.Code) : Nat.Partrec.Code := match c with
+def substPartrec (c : Code) (c' : Partrec.Code) : Partrec.Code := match c with
 | zero => .zero
 | succ => .succ
 | left => .left
@@ -86,43 +87,102 @@ theorem primrec₂_subst : Primrec₂ subst := by
 `substPartrec` is primitive recursive.
 -/
 theorem primrec₂_substPartrec : Primrec₂ substPartrec := by
-  refine (primrec_recOn (α := Code × Nat.Partrec.Code) (σ := Nat.Partrec.Code)
-    (pr := fun _ _ _ hf hg => Nat.Partrec.Code.pair hf hg)
-    (co := fun _ _ _ hf hg => Nat.Partrec.Code.comp hf hg)
-    (pc := fun _ _ _ hf hg => Nat.Partrec.Code.prec hf hg)
-    (rf := fun _ _ hf => Nat.Partrec.Code.rfind' hf)
+  refine (primrec_recOn (α := Code × Partrec.Code) (σ := Partrec.Code)
+    (pr := fun _ _ _ => Partrec.Code.pair)
+    (co := fun _ _ _ => Partrec.Code.comp)
+    (pc := fun _ _ _ => Partrec.Code.prec)
+    (rf := fun _ _ => Partrec.Code.rfind')
     Primrec.fst
     (.const .zero) (.const .succ) (.const .left) (.const .right)
     Primrec.snd
-    (Nat.Partrec.Code.primrec₂_pair.comp
-      (Primrec.fst.comp (Primrec.snd.comp (Primrec.snd.comp Primrec.snd)))
-      (Primrec.snd.comp (Primrec.snd.comp (Primrec.snd.comp Primrec.snd))))
-    (Nat.Partrec.Code.primrec₂_comp.comp
-      (Primrec.fst.comp (Primrec.snd.comp (Primrec.snd.comp Primrec.snd)))
-      (Primrec.snd.comp (Primrec.snd.comp (Primrec.snd.comp Primrec.snd))))
-    (Nat.Partrec.Code.primrec₂_prec.comp
-      (Primrec.fst.comp (Primrec.snd.comp (Primrec.snd.comp Primrec.snd)))
-      (Primrec.snd.comp (Primrec.snd.comp (Primrec.snd.comp Primrec.snd))))
-    (Nat.Partrec.Code.primrec_rfind'.comp (Primrec.snd.comp Primrec.snd))).of_eq ?_
+    (Partrec.Code.primrec₂_pair.comp
+      (.comp .fst (.comp .snd (.comp .snd .snd)))
+      (.comp .snd (.comp .snd (.comp .snd .snd))))
+    (Partrec.Code.primrec₂_comp.comp
+      (.comp .fst (.comp .snd (.comp .snd .snd)))
+      (.comp .snd (.comp .snd (.comp .snd .snd))))
+    (Partrec.Code.primrec₂_prec.comp
+      (.comp .fst (.comp .snd (.comp .snd .snd)))
+      (.comp .snd (.comp .snd (.comp .snd .snd))))
+    (Partrec.Code.primrec_rfind'.comp (.comp .snd .snd))).of_eq ?_
   intro ⟨c₁, c₂⟩
   induction c₁ with
   | zero | succ | left | right | oracle => rfl
-  | pair cf cg ihf ihg => exact congrArg₂ Nat.Partrec.Code.pair ihf ihg
-  | comp cf cg ihf ihg => exact congrArg₂ Nat.Partrec.Code.comp ihf ihg
-  | prec cf cg ihf ihg => exact congrArg₂ Nat.Partrec.Code.prec ihf ihg
-  | rfind' cf ihf => exact congrArg Nat.Partrec.Code.rfind' ihf
+  | pair cf cg ihf ihg => exact congrArg₂ Partrec.Code.pair ihf ihg
+  | comp cf cg ihf ihg => exact congrArg₂ Partrec.Code.comp ihf ihg
+  | prec cf cg ihf ihg => exact congrArg₂ Partrec.Code.prec ihf ihg
+  | rfind' cf ihf => exact congrArg Partrec.Code.rfind' ihf
 
 /--
 The `eval` of `c.subst c'` with oracle `o` is equal to the `eval` of `c` with oracle `c'.eval o`.
 -/
-theorem eval_subst (c c' : Code) (o : ℕ →. ℕ) : (c.subst c').eval o = c.eval (c'.eval o) := by
+lemma eval_subst (c c' : Code) (o : ℕ →. ℕ) : (c.subst c').eval o = c.eval (c'.eval o) := by
   induction c with simp [subst, eval, *]
 
 /--
 The `eval` of `c.substPartrec c'` is equal to the `eval` of `c` with oracle `c'.eval`.
 -/
-theorem eval_substPartrec (c : Code) (c' : Nat.Partrec.Code) : (c.substPartrec c').eval = c.eval c'.eval := by
-  induction c with simp [substPartrec, eval, Nat.Partrec.Code.eval, *]
+lemma eval_substPartrec (c : Code) (c' : Partrec.Code) : (c.substPartrec c').eval = c.eval c'.eval := by
+  induction c with simp [substPartrec, eval, Partrec.Code.eval, *]
+
+/--
+This essentially says that `(c.substPartrec c').evaln k` only uses the first `k` values of the oracle `c'`.
+
+Note: the more obvious conclusion `(c.substPartrec c₁).evaln k = (c.substPartrec c₂).evaln k` is false, since `c₁` and `c₂` can take a different number of steps, so it could be that `c₁` halts on some query while `c₂` does not.
+-/
+theorem evaln_substPartrec (c : Code) {c₁ c₂ : Partrec.Code} {k : ℕ} (hres : ∀ i < k, ∀ m ∈ c₁.eval i, m ∈ c₂.eval i) {n x₁ x₂} (hx₁ : x₁ ∈ (c.substPartrec c₁).evaln k n) (hx₂ : x₂ ∈ (c.substPartrec c₂).evaln k n) : x₁ = x₂ := by
+  induction k generalizing c n x₁ x₂ with
+  | zero => simp [Partrec.Code.evaln] at hx₁
+  | succ k IHk =>
+    have hres' : ∀ i < k, ∀ m ∈ c₁.eval i, m ∈ c₂.eval i :=
+      fun i hi => hres i (Nat.lt_succ_of_lt hi)
+    induction c generalizing n x₁ x₂ with
+    | zero | succ | left | right => simp_all [substPartrec]
+    | oracle =>
+      -- This is the only case where `hres` is used.
+      unfold substPartrec at hx₁ hx₂
+      have hn : n < k + 1 := Partrec.Code.evaln_bound hx₁
+      apply Partrec.Code.evaln_sound at hx₁
+      apply Partrec.Code.evaln_sound at hx₂
+      exact Part.mem_unique (hres n hn x₁ hx₁) hx₂
+    | pair cf cg IHcf IHcg =>
+      simp [substPartrec, Partrec.Code.evaln, Option.bind_eq_some_iff, Seq.seq] at hx₁ hx₂
+      obtain ⟨-, a₁, ha₁, b₁, hb₁, rfl⟩ := hx₁
+      obtain ⟨-, a₂, ha₂, b₂, hb₂, rfl⟩ := hx₂
+      rw [pair_eq_pair]
+      exact ⟨IHcf ha₁ ha₂, IHcg hb₁ hb₂⟩
+    | comp cf cg IHcf IHcg =>
+      simp [substPartrec, Partrec.Code.evaln, Option.bind_eq_some_iff] at hx₁ hx₂
+      obtain ⟨-, y₁, hy₁, hx₁⟩ := hx₁
+      obtain ⟨-, y₂, hy₂, hx₂⟩ := hx₂
+      rw [IHcg hy₁ hy₂] at hx₁
+      exact IHcf hx₁ hx₂
+    | prec cf cg IHcf IHcg =>
+      have := n.pair_unpair
+      generalize n.unpair.1 = a, n.unpair.2 = m at this
+      subst this
+      cases m with
+      | zero =>
+        simp [substPartrec, Partrec.Code.evaln, Option.bind_eq_some_iff] at hx₁ hx₂
+        exact IHcf hx₁.2 hx₂.2
+      | succ m =>
+        simp [substPartrec, Partrec.Code.evaln, Option.bind_eq_some_iff] at hx₁ hx₂
+        obtain ⟨-, y₁, hy₁, hx₁⟩ := hx₁
+        obtain ⟨-, y₂, hy₂, hx₂⟩ := hx₂
+        rw [← substPartrec] at hy₁ hy₂
+        rw [IHk _ hres' hy₁ hy₂] at hx₁
+        exact IHcg hx₁ hx₂
+    | rfind' cf IHcf =>
+      simp [substPartrec, Partrec.Code.evaln, Option.bind_eq_some_iff] at hx₁ hx₂
+      obtain ⟨-, y₁, hy₁, hx₁⟩ := hx₁
+      obtain ⟨-, y₂, hy₂, hx₂⟩ := hx₂
+      rw [IHcf hy₁ hy₂] at hx₁
+      cases y₂ with
+      | zero => simp_all
+      | succ y₂ =>
+        simp at hx₁ hx₂
+        rw [← substPartrec] at hx₁ hx₂
+        exact IHk _ hres' hx₁ hx₂
 
 end Nat.RecursiveIn.Code
 
